Define machine model, write prefancy->fancy pass, and prove Montgomery code correct

src/Experiments/SimplyTypedArithmetic.v
@@ -126,6 +126,9 @@ Module Associational.
       push; [|rewrite IHp]; reflexivity.
   Qed.
 
+  Lemma eval_rev p : eval (rev p) = eval p.
+  Proof. induction p; cbn [rev]; push; lia. Qed.
+
   Section Carries.
     Definition carryterm (w fw:Z) (t:Z * Z) :=
       if (Z.eqb (fst t) w)
@@ -1758,6 +1761,7 @@ Module BaseConversion.
          @Associational.eval_carry
          @Associational.eval_mul
          @Positional.eval_to_associational
+         Associational.eval_carryterm
          @eval_convert_bases using solve [auto using Z.positive_is_nonzero] : push_eval.
 
     Ltac push_eval := intros; autorewrite with push_eval; auto with zarith.
@@ -1767,14 +1771,30 @@ Module BaseConversion.
       let p' := convert_bases n m p in
       Positional.to_associational dw m p'.
 
+    (* TODO : move to Associational? *)
+    Section reorder.
+      Definition reordering_carry (w fw : Z) (p : list (Z * Z)) :=
+        fold_right (fun t acc =>
+                      let r := Associational.carryterm w fw t in
+                      if fst t =? w then acc ++ r else r ++ acc) nil p.
+
+      Lemma eval_reordering_carry w fw p (_:fw<>0):
+        Associational.eval (reordering_carry w fw p) = Associational.eval p.
+      Proof.
+        cbv [reordering_carry]. induction p; [reflexivity |].
+        autorewrite with push_fold_right. break_match; push_eval.
+      Qed.
+    End reorder.
+    Hint Rewrite eval_reordering_carry using solve [auto using Z.positive_is_nonzero] : push_eval.
+
     (* carry at specified indices in dw, then use Rows.flatten to convert to Positional with sw *)
     Definition from_associational idxs n (p : list (Z * Z)) : list Z :=
       (* important not to use Positional.carry here; we don't want to accumulate yet *)
-      let p' := fold_right (fun i acc => Associational.carry (dw i) (dw (S i) / dw i) acc) (Associational.bind_snd p) (rev idxs) in
+      let p' := fold_right (fun i acc => reordering_carry (dw i) (dw (S i) / dw i) acc) (Associational.bind_snd p) (rev idxs) in
       fst (Rows.flatten sw n (Rows.from_associational sw n p')).
 
     Lemma eval_carries p idxs :
-      Associational.eval (fold_right (fun i acc => Associational.carry (dw i) (dw (S i) / dw i) acc) p idxs) =
+      Associational.eval (fold_right (fun i acc => reordering_carry (dw i) (dw (S i) / dw i) acc) p idxs) =
       Associational.eval p.
     Proof. apply fold_right_invariant; push_eval. Qed.
     Hint Rewrite eval_carries: push_eval.
@@ -1821,7 +1841,7 @@ Module BaseConversion.
            As from_associational_inlined_correct.
     Proof.
       intros.
-      cbv beta iota delta [from_associational Associational.carry Associational.carryterm].
+      cbv beta iota delta [from_associational reordering_carry Associational.carryterm].
       cbv beta iota delta [Let_In]. (* inlines all shifts/lands from carryterm *)
       cbv beta iota delta [from_associational Rows.from_associational Columns.from_associational].
       cbv beta iota delta [Let_In]. (* inlines the shifts from place *)
@@ -1908,9 +1928,6 @@ Module BaseConversion.
       Z.rewrite_mod_small. reflexivity.
     Qed.
 
-    (* For some reason, this is a universe inconsistency if not factored out *)
-    Lemma nout_nonzero : nout <> 0%nat. Proof. omega. Qed.
-
     Derive widemul_inlined
            SuchThat (forall a b,
                         0 <= a * b < 2^log2base * 2^log2base ->
@@ -1922,8 +1939,32 @@ Module BaseConversion.
       cbv beta iota delta [widemul mul_converted].
       rewrite <-to_associational_inlined_correct with (p:=[a]).
       rewrite <-to_associational_inlined_correct with (p:=[b]).
-      rewrite <-from_associational_inlined_correct by (apply nout_nonzero || assumption).
+      rewrite <-from_associational_inlined_correct.
       subst widemul_inlined; reflexivity.
+    Qed.
+
+    Derive widemul_inlined_reverse
+           SuchThat (forall a b,
+                        0 <= a * b < 2^log2base * 2^log2base ->
+                        widemul_inlined_reverse a b = [(a * b) mod 2^log2base; (a * b) / 2^log2base])
+           As widemul_inlined_reverse_correct.
+    Proof.
+      intros.
+      rewrite <-widemul_inlined_correct by assumption.
+      cbv [widemul_inlined].
+      match goal with |- _ = from_associational_inlined sw dw ?idxs ?n ?p =>
+                      transitivity (from_associational_inlined sw dw idxs n (rev p));
+                        [ | transitivity (from_associational sw dw idxs n p); [ | reflexivity ] ](* reverse to make addc chains line up *)
+      end.
+      Focus 2. {
+        rewrite from_associational_inlined_correct by (subst nout; auto).
+        cbv [from_associational].
+        rewrite !Rows.flatten_partitions' by eauto using Rows.length_from_associational.
+        rewrite !Rows.eval_from_associational by (subst nout; auto).
+        f_equal.
+        rewrite !eval_carries, !Associational.bind_snd_correct, !Associational.eval_rev by auto.
+        reflexivity. } Unfocus.
+      subst widemul_inlined_reverse; reflexivity.
     Qed.
   End widemul.
 End BaseConversion.
@@ -8187,8 +8228,8 @@ Module Straightline.
 
     Section interp.
       Context {ident : type -> type -> Type} {interp_ident : forall s d, ident s d -> type.interp s -> type.interp d}.
+      Context {interp_cast : zrange -> Z -> Z}.
 
-      Definition interp_cast (r : zrange) (x : Z) : Z := ident.cast ident.cast_outside_of_range r x.
       Definition interp_cast2 (r : zrange * zrange) (x : Z * Z) : Z * Z :=
         (interp_cast (fst r) (fst x), interp_cast (snd r) (snd x)).
 
@@ -8220,9 +8261,10 @@ Module Straightline.
     End interp.
 
     Section proofs.
-      Local Notation straightline_interp := (expr.interp (ident:=default.ident) (interp_ident:=@ident.interp)).
+      Local Notation straightline_interp := (expr.interp (ident:=default.ident) (interp_ident:=@ident.interp) (interp_cast:=ident.cast (@ident.cast_outside_of_range))).
       Local Notation uinterp := (Uncurried.expr.interp (@ident.interp)).
       Local Notation uexpr := (@Uncurried.expr.expr ident type.interp).
+      Local Notation interp_scalar := (interp_scalar (interp_cast:=ident.cast (@ident.cast_outside_of_range))).
 
       Inductive ok_scalar_ident : forall {s d}, ident.ident s d -> Prop :=
       | ok_si_cast : forall r, ok_scalar_ident (ident.Z.cast r)
@@ -8273,11 +8315,11 @@ Module Straightline.
       .
 
       Lemma interp_cast_correct r (x : uexpr type.Z) :
-        interp_cast r (uinterp x) = uinterp (AppIdent (ident.Z.cast r) x).
+        ident.cast ident.cast_outside_of_range r (uinterp x) = uinterp (AppIdent (ident.Z.cast r) x).
       Proof. reflexivity. Qed.
 
       Lemma interp_cast2_correct r (x : uexpr (type.prod type.Z type.Z)) :
-        interp_cast2 r (uinterp x) = uinterp (AppIdent (ident.Z.cast2 r) x).
+        @interp_cast2 (ident.cast ident.cast_outside_of_range) r (uinterp x) = uinterp (AppIdent (ident.Z.cast2 r) x).
       Proof. cbn; break_match; reflexivity. Qed.
 
       Ltac invert H :=
@@ -8542,6 +8584,28 @@ Module PreFancy.
         apply BinInt.Z.mul_div_le; omega. }
     Qed.
 
+    Lemma wordmax_half_bits_le_wordmax : wordmax_half_bits <= wordmax.
+    Proof.
+      subst wordmax half_bits wordmax_half_bits.
+      apply Z.pow_le_mono_r; [lia|].
+      apply Z.div_le_upper_bound; lia.
+    Qed.
+
+    Lemma ones_half_bits : wordmax_half_bits - 1 = Z.ones half_bits.
+    Proof.
+      subst wordmax_half_bits. cbv [Z.ones].
+      rewrite Z.shiftl_mul_pow2, <-Z.sub_1_r by auto using half_bits_nonneg.
+      lia.
+    Qed.
+
+    Lemma wordmax_half_bits_squared : wordmax_half_bits * wordmax_half_bits = wordmax.
+    Proof.
+      subst wordmax half_bits wordmax_half_bits.
+      rewrite <-Z.pow_add_r by Z.zero_bounds.
+      rewrite Z.add_diag, Z.mul_div_eq by omega.
+      f_equal; lia.
+    Qed.
+
     Section with_var.
       Context {var : type -> Type} (dummy_arrow : forall s d, var (type.arrow s d)) (consts : list Z).
       Local Notation Z := (type.type_primitive type.Z).
@@ -8580,7 +8644,7 @@ Module PreFancy.
         option (@scalar var Z) :=
         match e in scalar t return option (@scalar var Z) with
         | Cast r (Land n x) =>
-          if (lower r =? 0) && (upper r =? (wordmax_half_bits - 1)) && (n =? 2^half_bits-1)
+          if (lower r =? 0) && (upper r =? (wordmax_half_bits - 1)) && (n =? wordmax_half_bits-1)
           then Some x
           else None
         | _ => None
@@ -8764,6 +8828,9 @@ Module PreFancy.
     End with_var.
 
     Section interp.
+      Context {interp_cast : zrange -> Z -> Z}.
+      Local Notation interp_scalar := (interp_scalar (interp_cast:=interp_cast)).
+      Local Notation interp_cast2 := (interp_cast2 (interp_cast:=interp_cast)).
       Local Notation low x := (Z.land x (wordmax_half_bits - 1)).
       Local Notation high x := (x >> half_bits).
       Local Notation shift x imm := ((x << imm) mod wordmax).
@@ -8797,6 +8864,9 @@ Module PreFancy.
     Section proofs.
       Context (dummy_arrow : forall s d, type.interp (s -> d)%ctype) (consts : list Z)
               (consts_ok : forall x, In x consts -> 0 <= x <= wordmax - 1).
+      Context {interp_cast : zrange -> Z -> Z} {interp_cast_correct : forall r x, lower r <= x <= upper r -> interp_cast r x = x}.
+      Local Notation interp_scalar := (interp_scalar (interp_cast:=interp_cast)).
+      Local Notation interp_cast2 := (interp_cast2 (interp_cast:=interp_cast)).
 
       Local Notation word_range := (r[0~>wordmax-1])%zrange.
       Local Notation half_word_range := (r[0~>wordmax_half_bits-1])%zrange.
@@ -8979,7 +9049,7 @@ Module PreFancy.
       .
 
       Inductive ok_expr : forall {t}, @expr type.interp ident.ident t -> Prop :=
-      | ok_of_scalar : forall t s, @ok_expr t (Scalar s)
+      | ok_of_scalar : forall t s, ok_scalar s -> @ok_expr t (Scalar s)
       | ok_letin_z : forall s d r idc x f,
           ok_ident _ type.Z x r idc ->
           ok_scalar x ->
@@ -9018,23 +9088,15 @@ Module PreFancy.
       Lemma interp_cast_noop x r :
         @has_range type.Z r x ->
         interp_cast r x = x.
-      Proof.
-        cbv [has_range interp_cast ident.cast]; intros.
-        break_match;
-          try match goal with H : _ && _ = true |- _ => rewrite andb_true_iff in H; destruct H end;
-          try match goal with H : _ && _ = false |- _ => rewrite andb_false_iff in H; destruct H end;
-          Z.ltb_to_lt; omega.
-      Qed.
+      Proof. cbv [has_range]; intros; auto. Qed.
 
       Lemma interp_cast2_noop x r :
         @has_range (type.prod type.Z type.Z) r x ->
         interp_cast2 r x = x.
       Proof.
-        cbv [has_range interp_cast2 interp_cast ident.cast]; intros.
-        break_match; destruct x;
-          repeat match goal with H : _ && _ = true |- _ => rewrite andb_true_iff in H; destruct H end;
-          repeat match goal with H : _ && _ = false |- _ => rewrite andb_false_iff in H; destruct H end;
-          Z.ltb_to_lt; try omega; reflexivity.
+        cbv [has_range interp_cast2]; intros.
+        rewrite !interp_cast_correct by tauto.
+        destruct x; reflexivity.
       Qed.
 
       Lemma has_range_shiftr n (x : scalar type.Z) :
@@ -9440,8 +9502,8 @@ Module PreFancy.
         is_halved y ->
         ok_scalar (Pair x y) ->
         @has_range type.Z word_range (ident.interp ident.Z.mul (interp_scalar (Pair x y))) ->
-        interp (of_straightline_ident dummy_arrow consts ident.Z.mul t word_range (Pair x y) g) =
-        interp (g (ident.interp ident.Z.mul (interp_scalar (Pair x y)))).
+        @interp interp_cast _ (of_straightline_ident dummy_arrow consts ident.Z.mul t word_range (Pair x y) g) =
+        @interp interp_cast _ (g (ident.interp ident.Z.mul (interp_scalar (Pair x y)))).
       Proof.
         intros Hx Hy Hok ?; invert Hok; cbn [interp_scalar of_straightline_ident].
         destruct (is_halved_cases x Hx ltac:(assumption)) as [ [? [Pxlow [Pxhigh Pxi] ] ] | [? [Pxlow [Pxhigh Pxi] ] ] ];
@@ -9459,12 +9521,39 @@ Module PreFancy.
         intros. apply Z.mod_small; omega.
       Qed.
 
+      Lemma half_word_range_le_word_range r :
+        upper r = wordmax_half_bits - 1 ->
+        lower r = 0 ->
+        (r <=? word_range)%zrange = true.
+      Proof.
+        pose proof wordmax_half_bits_le_wordmax.
+        destruct r; cbv [is_tighter_than_bool ZRange.lower ZRange.upper].
+        intros; subst.
+        apply andb_true_iff; split; Z.ltb_to_lt; lia.
+      Qed.
+
+      Lemma and_shiftl_half_bits_eq x :
+        (x &' (wordmax_half_bits - 1)) << half_bits = x << half_bits mod wordmax.
+      Proof.
+        rewrite ones_half_bits.
+        rewrite Z.land_ones, !Z.shiftl_mul_pow2 by auto using half_bits_nonneg.
+        rewrite <-wordmax_half_bits_squared.
+        subst wordmax_half_bits.
+        rewrite Z.mul_mod_distr_r_full.
+        reflexivity.
+      Qed.
+
+      Lemma in_word_range_word_range : in_word_range word_range.
+      Proof.
+        cbv [in_word_range is_tighter_than_bool].
+        rewrite !Z.leb_refl; reflexivity.
+      Qed.
+
       Lemma invert_shift_correct (s : scalar type.Z) x imm :
         ok_scalar s ->
         invert_shift consts s = Some (x, imm) ->
         interp_scalar s = (interp_scalar x << imm) mod wordmax.
       Proof.
-        (*
         intros Hok ?; invert Hok;
           try match goal with H : ok_scalar ?x, H' : context[Cast _ ?x] |- _ =>
                           invert H end;
@@ -9472,44 +9561,34 @@ Module PreFancy.
                           invert H end;
           try match goal with H : ok_scalar ?x, H' : context[Shiftl _ (Cast _ ?x)] |- _ =>
                           invert H end;
-          try (cbn [invert_shift invert_upper invert_upper'] in *; discriminate).
-        {
+          try (cbn [invert_shift invert_upper invert_upper'] in *; discriminate);
           repeat match goal with
-                 | _ => progress (cbn [invert_shift invert_upper invert_upper'
-                                                    interp_scalar fst snd] in * )
-                 | _ => rewrite interp_cast_noop by eauto using has_range_loosen
-                 | H : ok_scalar (Shiftr _ _) |- _ => apply has_range_interp_scalar in H
-                 | H : context [if ?x then _ else _] |- _ =>
-                   let Heq := fresh in case_eq x; intro Heq; rewrite Heq in H
-                 | H : _ |- _ => rewrite andb_true_iff in H; destruct H; Z.ltb_to_lt
-                 | H : Some _ = Some _ |- _ => progress (invert H)
-                 | _ => progress subst
-                 | _ => reflexivity
-                 | _ => discriminate
-                 end.
-          rewrite has_word_range_mod_small.
-          2:eauto using has_range_loosen.
-        }
-        {
-          repeat match goal with
-                 | _ => progress (cbn [invert_shift invert_upper invert_upper'
-                                                    invert_lower invert_lower'
-                                                    interp_scalar fst snd] in * )
-                 | _ => rewrite interp_cast_noop by eauto using has_range_loosen
+                 | _ => progress (cbn [invert_shift invert_lower invert_lower' invert_upper invert_upper' interp_scalar fst snd] in * )
+                 | _ => rewrite interp_cast_noop by eauto using has_half_word_range_land, has_half_word_range_shiftr, in_word_range_word_range, has_range_loosen
                  | H : ok_scalar (Shiftr _ _) |- _ => apply has_range_interp_scalar in H
                  | H : ok_scalar (Shiftl _ _) |- _ => apply has_range_interp_scalar in H
                  | H : ok_scalar (Land _ _) |- _ => apply has_range_interp_scalar in H
                  | H : context [if ?x then _ else _] |- _ =>
                    let Heq := fresh in case_eq x; intro Heq; rewrite Heq in H
+                 | H : context [match @constant_to_scalar ?v ?consts ?x with _ => _ end] |- _ =>
+                   let Heq := fresh in
+                   case_eq (@constant_to_scalar v consts x); intros until 0; intro Heq; rewrite Heq in *; [|discriminate];
+                     destruct (constant_to_scalar_cases _ _ Heq) as [ [? [? ?] ] | [? [? ?] ] ]; subst;
+                       pose proof (ok_scalar_constant_to_scalar _ _ Heq)
+                 | H : constant_to_scalar _ _ = Some _ |- _ => erewrite <-(constant_to_scalar_correct _ _ H)
                  | H : _ |- _ => rewrite andb_true_iff in H; destruct H; Z.ltb_to_lt
                  | H : Some _ = Some _ |- _ => progress (invert H)
+                 | _ => rewrite has_word_range_mod_small by eauto using has_range_loosen, half_word_range_le_word_range
+                 | _ => rewrite has_word_range_mod_small by
+                       (eapply has_range_loosen with (r1:=half_word_range);
+                        [ eapply has_half_word_range_shiftr with (r:=word_range) | ];
+                        eauto using in_word_range_word_range, half_word_range_le_word_range)
+                 | _ => rewrite and_shiftl_half_bits_eq
                  | _ => progress subst
                  | _ => reflexivity
                  | _ => discriminate
                  end.
       Qed.
-         *)
-        Admitted.
 
       Local Ltac solve_commutative_replace :=
         match goal with
@@ -9521,8 +9600,8 @@ Module PreFancy.
       Lemma of_straightline_ident_correct s d t x r (idc : ident.ident s d) g :
         ok_ident s d x r idc ->
         ok_scalar x ->
-        interp (of_straightline_ident dummy_arrow consts idc t r x g) =
-        interp (g (ident.interp idc (interp_scalar x))).
+        @interp interp_cast _ (of_straightline_ident dummy_arrow consts idc t r x g) =
+        @interp interp_cast _ (g (ident.interp idc (interp_scalar x))).
       Proof.
         intros.
         pose proof wordmax_half_bits_pos.
@@ -9559,7 +9638,8 @@ Module PreFancy.
 
       Lemma of_straightline_correct {t} (e : expr t) :
         ok_expr e ->
-        interp (of_straightline dummy_arrow consts e) = Straightline.expr.interp (interp_ident:=@ident.interp) e.
+        @interp interp_cast _ (of_straightline dummy_arrow consts e)
+        = Straightline.expr.interp (interp_ident:=@ident.interp) (interp_cast:=interp_cast) e.
       Proof.
         induction 1; cbn [of_straightline]; intros;
           repeat match goal with
@@ -9572,11 +9652,78 @@ Module PreFancy.
                  end.
       Qed.
     End proofs.
+
+   Section no_interp_cast.
+      Context (dummy_arrow : forall s d, type.interp (s -> d)%ctype) (consts : list Z)
+              (consts_ok : forall x, In x consts -> 0 <= x <= wordmax - 1).
+
+      Local Arguments interp _ {_} _.
+      Local Arguments interp_scalar _ {_} _.
+
+      Local Ltac tighter_than_to_le :=
+        repeat match goal with
+               | _ => progress (cbv [is_tighter_than_bool] in * )
+               | _ => rewrite andb_true_iff in *
+               | H : _ /\ _ |- _ => destruct H
+               end; Z.ltb_to_lt.
+
+      Lemma replace_interp_cast_scalar {t} (x : scalar t) interp_cast interp_cast'
+        (interp_cast_correct : forall r x, lower r <= x <= upper r -> interp_cast r x = x)
+        (interp_cast'_correct : forall r x, lower r <= x <= upper r -> interp_cast' r x = x) :
+        ok_scalar x ->
+        interp_scalar interp_cast x = interp_scalar interp_cast' x.
+      Proof.
+        induction 1; cbn [interp_scalar Straightline.expr.interp_scalar];
+          repeat match goal with
+                 | _ => progress (cbv [has_range interp_cast2] in * )
+                 | _ => progress tighter_than_to_le
+                 | H : ok_scalar _ |- _ => apply (has_range_interp_scalar (interp_cast_correct:=interp_cast_correct)) in H
+                 | _ => rewrite <-IHok_scalar
+                 | _ => rewrite interp_cast_correct by omega
+                 | _ => rewrite interp_cast'_correct by omega
+                 | _ => congruence
+                 end.
+      Qed.
+
+      Lemma replace_interp_cast {t} (e : expr t) interp_cast interp_cast'
+        (interp_cast_correct : forall r x, lower r <= x <= upper r -> interp_cast r x = x)
+        (interp_cast'_correct : forall r x, lower r <= x <= upper r -> interp_cast' r x = x) :
+        ok_expr consts e ->
+        interp interp_cast (of_straightline dummy_arrow consts e) =
+        interp interp_cast' (of_straightline dummy_arrow consts e).
+      Proof.
+        induction 1; intros; cbn [of_straightline interp].
+        { apply replace_interp_cast_scalar; auto. }
+        { rewrite !of_straightline_ident_correct by auto.
+          rewrite replace_interp_cast_scalar with (interp_cast'0:=interp_cast') by auto.
+          eauto using ident_interp_has_range. }
+        { rewrite !of_straightline_ident_correct by auto.
+          rewrite replace_interp_cast_scalar with (interp_cast'0:=interp_cast') by auto.
+          eauto using ident_interp_has_range. }
+      Qed.
+    End no_interp_cast.
   End with_wordmax.
 
   Definition of_Expr {s d} (log2wordmax : Z) (consts : list Z) (e : Expr (s -> d))
              (var : type -> Type) (x : var s) dummy_arrow : @Straightline.expr.expr var ident d :=
     @of_straightline log2wordmax var dummy_arrow consts _ (Straightline.of_Expr e var x dummy_arrow).
+
+  Definition interp_cast_mod w r x := if (lower r =? 0)
+                                      then if (upper r =? 2^w - 1)
+                                           then x mod (2^w)
+                                           else if (upper r =? 1)
+                                                then x mod 2
+                                                else x
+                                      else x.
+
+  Lemma interp_cast_mod_correct w r x :
+    lower r <= x <= upper r ->
+    interp_cast_mod w r x = x.
+  Proof.
+    cbv [interp_cast_mod].
+    intros; break_match; rewrite ?andb_true_iff in *; intuition; Z.ltb_to_lt;
+      apply Z.mod_small; omega.
+  Qed.
 
   Lemma of_Expr_correct {s d} (log2wordmax : Z) (consts : list Z) (e : Expr (s -> d))
         (e' : (type.interp s -> Uncurried.expr.expr d))
@@ -9589,11 +9736,14 @@ Module PreFancy.
     ok_expr log2wordmax consts
             (of_uncurried (dummy_arrow:=dummy_arrow) (depth (fun _ : type => unit) (fun _ : type => tt) (e _)) (e' x)) ->
     (depth type.interp (@DefaultValue.type.default) (e' x) <= depth (fun _ : type => unit) (fun _ : type => tt) (e _))%nat ->
-    interp log2wordmax (of_Expr log2wordmax consts e type.interp x dummy_arrow) = @Uncurried.expr.interp _ (@ident.interp) _ (e type.interp) x.
+    @interp log2wordmax (interp_cast_mod log2wordmax) _ (of_Expr log2wordmax consts e type.interp x dummy_arrow) = @Uncurried.expr.interp _ (@ident.interp) _ (e type.interp) x.
   Proof.
     intro He'; intros; cbv [of_Expr Straightline.of_Expr].
     rewrite He'; cbn [invert_Abs expr.interp].
-    rewrite of_straightline_correct by assumption.
+    assert (forall r z, lower r <= z <= upper r -> ident.cast ident.cast_outside_of_range r z = z) as interp_cast_correct.
+    { cbv [ident.cast]; intros; break_match; rewrite ?andb_true_iff, ?andb_false_iff in *; intuition; Z.ltb_to_lt; omega. }
+    erewrite replace_interp_cast with (interp_cast':=ident.cast ident.cast_outside_of_range) by auto using interp_cast_mod_correct.
+    rewrite of_straightline_correct by auto.
     erewrite Straightline.expr.of_uncurried_correct by eassumption.
     reflexivity.
   Qed.
@@ -9650,6 +9800,661 @@ Module PreFancy.
     Notation "( x , y )" := (Pair x y) (at level 10, left associativity).
   End Notations.
 End PreFancy.
+
+Module Fancy.
+  Import Straightline.expr.
+
+  Module CC.
+    Inductive code : Type :=
+    | C : code
+    | M : code
+    | L : code
+    | Z : code
+    .
+
+    Record state :=
+      { cc_c : bool; cc_m : bool; cc_l : bool; cc_z : bool }.
+
+    Definition code_dec (x y : code) : {x = y} + {x <> y}.
+    Proof. destruct x, y; try apply (left eq_refl); right; congruence. Defined.
+
+    Definition update (to_write : list code) (result : BinInt.Z) (cc_spec : code -> BinInt.Z -> bool) (old_state : state)
+      : state :=
+      {|
+        cc_c := if (In_dec code_dec C to_write)
+                then cc_spec C result
+                else old_state.(cc_c);
+        cc_m := if (In_dec code_dec M to_write)
+                then cc_spec M result
+                else old_state.(cc_m);
+        cc_l := if (In_dec code_dec L to_write)
+                then cc_spec L result
+                else old_state.(cc_l);
+        cc_z := if (In_dec code_dec Z to_write)
+                then cc_spec Z result
+                else old_state.(cc_z)
+      |}.
+
+  End CC.
+
+  Record instruction :=
+    {
+      num_source_regs : nat;
+      writes_conditions : list CC.code;
+      spec : tuple Z num_source_regs -> CC.state -> Z
+    }.
+
+  Section expr.
+    Context {name : Type} (name_eqb : name -> name -> bool) (wordmax : Z) (cc_spec : CC.code -> Z -> bool).
+
+    Inductive expr :=
+    | Ret : name -> expr
+    | Instr (i : instruction)
+            (rd : name) (* destination register *)
+            (args : tuple name i.(num_source_regs)) (* source registers *)
+            (cont : expr) (* next line *)
+      : expr
+    .
+
+    Fixpoint interp (e : expr) (cc : CC.state) (ctx : name -> Z) : Z :=
+      match e with
+      | Ret n => ctx n
+      | Instr i rd args cont =>
+        let result := i.(spec) (Tuple.map ctx args) cc in
+        let new_cc := CC.update i.(writes_conditions) result cc_spec cc in
+        let new_ctx := (fun n : name => if name_eqb n rd then result mod wordmax else ctx n) in
+        interp cont new_cc new_ctx
+      end.
+  End expr.
+
+  Section ISA.
+    Import CC.
+
+    (* For the C flag, we have to consider cases with a negative result (like the one returned by an underflowing borrow).
+       In these cases, we want to set the C flag to true. *)
+    Definition cc_spec (x : CC.code) (result : BinInt.Z) : bool :=
+      match x with
+      | CC.C => if result <? 0 then true else Z.testbit result 256
+      | CC.M => Z.testbit result 255
+      | CC.L => Z.testbit result 0
+      | CC.Z => result =? 0
+      end.
+
+    Local Definition lower128 x := (Z.land x (Z.ones 128)).
+    Local Definition upper128 x := (Z.shiftr x 128).
+    Local Notation "x '[C]'" := (if x.(cc_c) then 1 else 0) (at level 20).
+    Local Notation "x '[M]'" := (if x.(cc_m) then 1 else 0) (at level 20).
+    Local Notation "x '[L]'" := (if x.(cc_l) then 1 else 0) (at level 20).
+    Local Notation "x '[Z]'" := (if x.(cc_z) then 1 else 0) (at level 20).
+    Local Notation "'int'" := (BinInt.Z).
+    Local Notation "x << y" := ((x << y) mod (2^256)) : Z_scope. (* truncating left shift *)
+
+
+    (* Note: In the specification document, argument order gets a bit
+    confusing. Like here, r0 is always the first argument "source 0"
+    and r1 the second. But the specification of MUL128LU is:
+            (R[RS1][127:0] * R[RS0][255:128])
+
+    while the specification of SUB is:
+          (R[RS0] - shift(R[RS1], imm))
+
+    In the SUB case, r0 is really treated the first argument, but in
+    MUL128LU the order seems to be reversed; rather than low-high, we
+    take the high part of the first argument r0 and the low parts of
+    r1. This is also true for MUL128UL. *)
+
+    Definition ADD (imm : int) : instruction :=
+      {|
+        num_source_regs := 2;
+        writes_conditions := [C; M; L; Z];
+        spec := (fun '(r0, r1) cc =>
+                   r0 + (r1 << imm))
+      |}.
+
+    Definition ADDC (imm : int) : instruction :=
+      {|
+        num_source_regs := 2;
+        writes_conditions := [C; M; L; Z];
+        spec := (fun '(r0, r1) cc =>
+                   r0 + (r1 << imm) + cc[C])
+      |}.
+
+    Definition SUB (imm : int) : instruction :=
+      {|
+        num_source_regs := 2;
+        writes_conditions := [C; M; L; Z];
+        spec := (fun '(r0, r1) cc =>
+                   r0 - (r1 << imm))
+      |}.
+
+    Definition MUL128LL : instruction :=
+      {|
+        num_source_regs := 2;
+        writes_conditions := [M; L; Z];
+        spec := (fun '(r0, r1) cc =>
+                   (lower128 r0) * (lower128 r1))
+      |}.
+
+    Definition MUL128LU : instruction :=
+      {|
+        num_source_regs := 2;
+        writes_conditions := [M; L; Z];
+        spec := (fun '(r0, r1) cc =>
+                   (lower128 r1) * (upper128 r0)) (* see note *)
+      |}.
+
+    Definition MUL128UL : instruction :=
+      {|
+        num_source_regs := 2;
+        writes_conditions := [M; L; Z];
+        spec := (fun '(r0, r1) cc =>
+                   (upper128 r1) * (lower128 r0)) (* see note *)
+      |}.
+
+    Definition MUL128UU : instruction :=
+      {|
+        num_source_regs := 2;
+        writes_conditions := [M; L; Z];
+        spec := (fun '(r0, r1) cc =>
+                   (upper128 r0) * (upper128 r1))
+      |}.
+
+    Definition RSHI (imm : int) : instruction :=
+      {|
+        num_source_regs := 2;
+        writes_conditions := [M; L; Z];
+        spec := (fun '(r0, r1) cc =>
+                   (r0 + (r1 << 256)) >> imm)
+      |}.
+
+    Definition SELC : instruction :=
+      {|
+        num_source_regs := 2;
+        writes_conditions := [];
+        spec := (fun '(r0, r1) cc =>
+                   if cc[C] =? 1 then r0 else r1)
+      |}.
+
+    Definition SELM : instruction :=
+      {|
+        num_source_regs := 2;
+        writes_conditions := [];
+        spec := (fun '(r0, r1) cc =>
+                   if cc[M] =? 1 then r0 else r1)
+      |}.
+
+    Definition SELL : instruction :=
+      {|
+        num_source_regs := 2;
+        writes_conditions := [];
+        spec := (fun '(r0, r1) cc =>
+                   if cc[L] =? 1 then r0 else r1)
+      |}.
+
+    (* TODO : treat the MOD register specially, like CC *)
+    Definition ADDM : instruction :=
+      {|
+        num_source_regs := 3;
+        writes_conditions := [M; L; Z];
+        spec := (fun '(r0, r1, MOD) cc =>
+                   let ra := r0 + r1 in
+                   if ra >=? MOD
+                   then ra - MOD
+                   else ra)
+      |}.
+
+  End ISA.
+
+  Module Registers.
+    Inductive register : Type :=
+    | r0 : register
+    | r1 : register
+    | r2 : register
+    | r3 : register
+    | r4 : register
+    | r5 : register
+    | r6 : register
+    | r7 : register
+    | r8 : register
+    | r9 : register
+    | r10 : register
+    | r11 : register
+    | r12 : register
+    | r13 : register
+    | r14 : register
+    | r15 : register
+    | r16 : register
+    | r17 : register
+    | r18 : register
+    | r19 : register
+    | r20 : register
+    | r21 : register
+    | r22 : register
+    | r23 : register
+    | r24 : register
+    | r25 : register
+    | r26 : register
+    | r27 : register
+    | r28 : register
+    | r29 : register
+    | r30 : register
+    | RegZero : register (* r31 *)
+    | RegMod : register
+    .
+
+    Definition reg_dec (x y : register) : {x = y} + {x <> y}.
+    Proof. destruct x, y; try (apply left; congruence); right; congruence. Defined.
+    Definition reg_eqb x y := if reg_dec x y then true else false.
+
+    Lemma reg_eqb_neq x y : x <> y -> reg_eqb x y = false.
+    Proof. cbv [reg_eqb]; break_match; congruence. Qed.
+    Lemma reg_eqb_refl x : reg_eqb x x = true.
+    Proof. cbv [reg_eqb]; break_match; congruence. Qed.
+  End Registers.
+
+  Section of_prefancy.
+    Context (name : Type) (name_succ : name -> name) (error : name) (consts : Z -> option name).
+
+    Fixpoint var (t : type) : Type :=
+      match t with
+      | type.type_primitive type.Z => name
+      | type.prod a b => var a * var b
+      | _ => unit
+      end.
+
+    Fixpoint of_prefancy_scalar {t} (s : @scalar var t) : var t :=
+      match s with
+      | Var t v => v
+      | Pair a b x y => (of_prefancy_scalar x, of_prefancy_scalar y)
+      | Cast r x => of_prefancy_scalar x
+      | Cast2 r x => of_prefancy_scalar x
+      | Fst a b x => fst (of_prefancy_scalar x)
+      | Snd a b x => snd (of_prefancy_scalar x)
+      | Shiftr n x => error
+      | Shiftl n x => error
+      | Land n x => error
+      | CC_m n x => error
+      | @Primitive _ type.Z x => match consts x with
+                                 | Some n => n
+                                 | None => error
+                                 end
+      | @Primitive _ _ x => tt
+      | TT => tt
+      | Nil _ => tt
+      end.
+
+    (* Note : some argument orders are reversed for MUL128LU, MUL128UL, SELC, SELM, and SELL *)
+    Definition of_prefancy_ident {s d} (idc : PreFancy.ident s d)
+      : @scalar var s -> {i : instruction & tuple name i.(num_source_regs) } :=
+      match idc in PreFancy.ident s d return _ with
+      | PreFancy.add imm => fun args : @scalar var (type.Z * type.Z) =>
+                              existT _ (ADD imm) (of_prefancy_scalar args)
+      | PreFancy.addc imm => fun args : @scalar var (type.Z * type.Z * type.Z) =>
+                               existT _ (ADDC imm) (of_prefancy_scalar (Pair (Snd (Fst args)) (Snd args)))
+      | PreFancy.sub imm => fun args : @scalar var (type.Z * type.Z) =>
+                              existT _ (SUB imm) (of_prefancy_scalar args)
+      | PreFancy.mulll => fun args : @scalar var (type.Z * type.Z) =>
+                            existT _ MUL128LL (of_prefancy_scalar args)
+      | PreFancy.mullh => fun args : @scalar var (type.Z * type.Z) =>
+                            existT _ MUL128LU (of_prefancy_scalar (Pair (Snd args) (Fst args)))
+      | PreFancy.mulhl => fun args : @scalar var (type.Z * type.Z) =>
+                            existT _ MUL128UL (of_prefancy_scalar (Pair (Snd args) (Fst args)))
+      | PreFancy.mulhh => fun args : @scalar var (type.Z * type.Z) =>
+                            existT _ MUL128UU (of_prefancy_scalar args)
+      | PreFancy.rshi imm => fun args : @scalar var (type.Z * type.Z) =>
+                               existT _ (RSHI imm) (of_prefancy_scalar args)
+      | PreFancy.selc => fun args : @scalar var (type.Z * type.Z * type.Z) =>
+                           existT _ SELC (of_prefancy_scalar (Pair (Snd args) (Snd (Fst args))))
+      | PreFancy.selm => fun args : @scalar var (type.Z * type.Z * type.Z) =>
+                           existT _ SELM (of_prefancy_scalar (Pair (Snd args) (Snd (Fst args))))
+      | PreFancy.sell => fun args : @scalar var (type.Z * type.Z * type.Z) =>
+                           existT _ SELL (of_prefancy_scalar (Pair (Snd args) (Snd (Fst args))))
+      | PreFancy.addm => fun args : @scalar var (type.Z * type.Z * type.Z) =>
+                           existT _ ADDM (of_prefancy_scalar args)
+      end.
+
+    Fixpoint of_prefancy (next_name : name) {t} (e : @Straightline.expr.expr var PreFancy.ident t) : expr :=
+      match e with
+      | LetInAppIdentZ s d r idc x f =>
+        let instr_args := @of_prefancy_ident s type.Z idc x in
+        let i : instruction := projT1 instr_args in
+        let args : tuple name i.(num_source_regs) := projT2 instr_args in
+        Instr i next_name args (of_prefancy (name_succ next_name) (f next_name))
+      | LetInAppIdentZZ s d r idc x f =>
+        let instr_args := @of_prefancy_ident s (type.Z * type.Z) idc x in
+        let i : instruction := projT1 instr_args in
+        let args : tuple name i.(num_source_regs) := projT2 instr_args in
+        Instr i next_name args (of_prefancy (name_succ next_name) (f (next_name, error))) (* we pass the error code as the carry register, because it cannot be read from directly. *)
+      | Scalar type.Z s => Ret (of_prefancy_scalar s)
+      | _ => Ret error
+      end.
+  End of_prefancy.
+
+  Section allocate_registers.
+    Context (reg name : Type) (name_eqb : name -> name -> bool) (error : reg).
+    Fixpoint allocate (e : @expr name) (reg_list : list reg) (name_to_reg : name -> reg) : @expr reg :=
+      match e with
+      | Ret n => Ret (name_to_reg n)
+      | Instr i rd args cont =>
+        match reg_list with
+        | r :: reg_list' => Instr i r (Tuple.map name_to_reg args) (allocate cont reg_list' (fun n => if name_eqb n rd then r else name_to_reg n))
+        | nil => Ret error
+        end
+      end.
+  End allocate_registers.
+
+  Definition test_prog : @expr positive :=
+    Instr (ADD (128)) 3%positive (1, 2)%positive
+          (Instr (ADDC 0) 4%positive (3,1)%positive
+                 (Ret 4%positive)).
+
+  Definition x1 := 2^256 - 1.
+  Definition x2 := 2^128 - 1.
+  Definition wordmax := 2^256.
+  Definition expected :=
+    let r3' := (x1 + (x2 << 128)) in
+    let r3 := r3' mod wordmax in
+    let c := r3' / wordmax in
+    let r4' := (r3 + x1 + c) in
+    r4' mod wordmax.
+  Definition actual :=
+    interp Pos.eqb
+           (2^256) cc_spec test_prog {|CC.cc_c:=false; CC.cc_m:=false; CC.cc_l:=false; CC.cc_z:=false|}
+           (fun n => if n =? 1%positive
+                     then x1
+                     else if n =? 2%positive
+                          then x2
+                          else 0).
+  Lemma test_prog_ok : expected = actual.
+  Proof. reflexivity. Qed.
+
+  Definition of_Expr {s d} next_name (consts : Z -> option positive) (consts_list : list Z) (e : Expr (s -> d)) (x : var positive s) dummy_arrow : positive -> @expr positive :=
+    fun error =>
+      @of_prefancy positive Pos.succ error consts next_name _ (PreFancy.of_Expr 256 consts_list e (var positive) x dummy_arrow).
+
+End Fancy.
+
+Module Prod.
+  Import Fancy. Import Registers.
+
+  Definition Mul256 (out src1 src2 tmp : register) (cont : Fancy.expr) : Fancy.expr :=
+    Instr MUL128LL out (src1, src2)
+          (Instr MUL128UL tmp (src1, src2)
+                 (Instr (ADD 128) out (out, tmp)
+                        (Instr MUL128LU tmp (src1, src2)
+                               (Instr (ADD 128) out (out, tmp) cont)))).
+  Definition Mul256x256 (out outHigh src1 src2 tmp : register) (cont : Fancy.expr) : Fancy.expr :=
+    Instr MUL128LL out (src1, src2)
+          (Instr MUL128UU outHigh (src1, src2)
+                 (Instr MUL128UL tmp (src1, src2)
+                        (Instr (ADD 128) out (out, tmp)
+                               (Instr (ADDC (-128)) outHigh (outHigh, tmp)
+                                      (Instr MUL128LU tmp (src1, src2)
+                                             (Instr (ADD 128) out (out, tmp)
+                                                    (Instr (ADDC (-128)) outHigh (outHigh, tmp) cont))))))).
+
+  Definition MontRed256 lo hi y t1 t2 scratch RegPInv : @Fancy.expr register :=
+    Mul256 y lo RegPInv t1
+           (Mul256x256 t1 t2 y RegMod scratch
+                       (Instr (ADD 0) lo (lo, t1)
+                              (Instr (ADDC 0) hi (hi, t2)
+                                     (Instr SELC y (RegMod, RegZero)
+                                            (Instr (SUB 0) lo (hi, y)
+                                                   (Instr ADDM lo (lo, RegZero, RegMod)
+                                                          (Ret lo))))))).
+End Prod.
+
+Module ProdEquiv.
+  Import Fancy. Import Registers.
+
+  Definition interp256 := Fancy.interp reg_eqb (2^256) cc_spec.
+  Lemma interp_step i rd args cont cc ctx :
+    interp256 (Instr i rd args cont) cc ctx =
+      let result := spec i (Tuple.map ctx args) cc in
+      let new_cc := CC.update (writes_conditions i) result cc_spec cc in
+      let new_ctx := fun n => if reg_eqb n rd then result mod wordmax else ctx n in interp256 cont new_cc new_ctx.
+  Proof. reflexivity. Qed.
+
+  (* TODO : move *)
+  Lemma tuple_map_ext {A B} (f g : A -> B) n (t : tuple A n) :
+    (forall x : A, f x = g x) ->
+    Tuple.map f t = Tuple.map g t.
+  Proof.
+    destruct n; [reflexivity|]; cbn in *.
+    induction n; cbn in *; intro H; auto; [ ].
+    rewrite IHn by assumption.
+    rewrite H; reflexivity.
+  Qed.
+
+  Lemma interp_state_equiv e :
+    forall cc ctx cc' ctx',
+    cc = cc' -> (forall r, ctx r = ctx' r) ->
+    interp256 e cc ctx = interp256 e cc' ctx'.
+  Proof.
+    induction e; intros; subst; cbn; [solve[auto]|].
+    apply IHe; rewrite tuple_map_ext with (g:=ctx') by auto;
+      [reflexivity|].
+    intros; break_match; auto.
+  Qed.
+  Lemma cc_overwrite_full x1 x2 l1 cc :
+    CC.update [CC.C; CC.M; CC.L; CC.Z] x2 cc_spec (CC.update l1 x1 cc_spec cc) = CC.update [CC.C; CC.M; CC.L; CC.Z] x2 cc_spec cc.
+  Proof.
+    cbv [CC.update]. cbn [CC.cc_c CC.cc_m CC.cc_l CC.cc_z].
+    break_match; try match goal with H : ~ In _ _ |- _ => cbv [In] in H; tauto end.
+    reflexivity.
+  Qed.
+
+  Lemma tuple_map_ext_In {A B} (f g : A -> B) n (t : tuple A n) :
+    (forall x, In x (to_list n t) -> f x = g x) ->
+    Tuple.map f t = Tuple.map g t.
+  Proof.
+    destruct n; [reflexivity|]; cbn in *.
+    induction n; cbn in *; intro H; auto; [ ].
+    destruct t.
+    rewrite IHn by auto using in_cons.
+    rewrite H; auto using in_eq.
+  Qed.
+
+  Definition value_unused r e : Prop :=
+    forall x cc ctx, interp256 e cc ctx = interp256 e cc (fun r' => if reg_eqb r' r then x else ctx r').
+
+  Lemma value_unused_skip r i rd args cont (Hcont: value_unused r cont) :
+    r <> rd ->
+    (~ In r (Tuple.to_list _ args)) ->
+    value_unused r (Instr i rd args cont).
+  Proof.
+    cbv [value_unused] in *; intros.
+    rewrite !interp_step; cbv zeta.
+    rewrite Hcont with (x:=x).
+    match goal with |- ?lhs = ?rhs =>
+                    match lhs with context [Tuple.map ?f ?t] =>
+                                   match rhs with context [Tuple.map ?g ?t] =>
+                                                  rewrite (tuple_map_ext_In f g) by (intros; cbv [reg_eqb]; break_match; congruence)
+                                   end end end.
+    apply interp_state_equiv; [ congruence | ].
+    { intros; cbv [reg_eqb] in *; break_match; congruence. }
+  Qed.
+
+  Lemma value_unused_overwrite r i args cont :
+    (~ In r (Tuple.to_list _ args)) ->
+    value_unused r (Instr i r args cont).
+  Proof.
+    cbv [value_unused]; intros; rewrite !interp_step; cbv zeta.
+    match goal with |- ?lhs = ?rhs =>
+                    match lhs with context [Tuple.map ?f ?t] =>
+                                   match rhs with context [Tuple.map ?g ?t] =>
+                                                  rewrite (tuple_map_ext_In f g) by (intros; cbv [reg_eqb]; break_match; congruence)
+                                   end end end.
+    apply interp_state_equiv; [ congruence | ].
+    { intros; cbv [reg_eqb] in *; break_match; congruence. }
+  Qed.
+
+  Lemma value_unused_ret r r' :
+    r <> r' ->
+    value_unused r (Ret r').
+  Proof.
+    cbv - [reg_dec]; intros.
+    break_match; congruence.
+  Qed.
+
+  Ltac remember_results :=
+    repeat match goal with |- context [(spec ?i ?args ?flags) mod ?w] =>
+                    let x := fresh "x" in
+                    let y := fresh "y" in
+                    let Heqx := fresh "Heqx" in
+                    remember (spec i args flags) as x eqn:Heqx;
+                    remember (x mod w) as y
+           end.
+
+  Ltac do_interp_step :=
+    rewrite interp_step; cbn - [interp spec];
+    repeat progress rewrite ?reg_eqb_neq, ?reg_eqb_refl by congruence;
+    remember_results.
+
+  Lemma interp_Mul256 out src1 src2 tmp tmp2 cont cc ctx:
+    out <> src1 ->
+    out <> src2 ->
+    out <> tmp ->
+    out <> tmp2 ->
+    src1 <> src2 ->
+    src1 <> tmp ->
+    src1 <> tmp2 ->
+    src2 <> tmp ->
+    src2 <> tmp2 ->
+    tmp <> tmp2 ->
+    value_unused tmp cont ->
+    value_unused tmp2 cont ->
+    interp256 (Prod.Mul256 out src1 src2 tmp cont) cc ctx =
+    interp256 (
+        Instr MUL128LU tmp (src1, src2)
+              (Instr MUL128UL tmp2 (src1, src2)
+                     (Instr MUL128LL out (src1, src2)
+                                 (Instr (ADD 128) out (out, tmp2)
+                                        (Instr (ADD 128) out (out, tmp) cont))))) cc ctx.
+  Proof.
+    intros; cbv [Prod.Mul256].
+    repeat (do_interp_step; cbn [spec MUL128LL MUL128UL MUL128LU ADD] in * ).
+
+    match goal with H : value_unused tmp _ |- _ => erewrite H end.
+    match goal with H : value_unused tmp2 _ |- _ => erewrite H end.
+    apply interp_state_equiv.
+    { rewrite !cc_overwrite_full.
+      f_equal. subst. lia. }
+    { intros; cbv [reg_eqb].
+      repeat (break_match_step ltac:(fun _ => idtac); try congruence); reflexivity. }
+  Qed.
+
+  Lemma interp_Mul256x256 out outHigh src1 src2 tmp tmp2 cont cc ctx:
+    out <> src1 ->
+    out <> outHigh ->
+    out <> src2 ->
+    out <> tmp ->
+    out <> tmp2 ->
+    outHigh <> src1 ->
+    outHigh <> src2 ->
+    outHigh <> tmp ->
+    outHigh <> tmp2 ->
+    src1 <> src2 ->
+    src1 <> tmp ->
+    src1 <> tmp2 ->
+    src2 <> tmp ->
+    src2 <> tmp2 ->
+    tmp <> tmp2 ->
+    value_unused tmp cont ->
+    value_unused tmp2 cont ->
+    interp256 (Prod.Mul256x256 out outHigh src1 src2 tmp cont) cc ctx =
+    interp256 (
+        Instr MUL128LL out (src1, src2)
+              (Instr MUL128LU tmp (src1, src2)
+                     (Instr MUL128UL tmp2 (src1, src2)
+                            (Instr MUL128UU outHigh (src1, src2)
+                                   (Instr (ADD 128) out (out, tmp2)
+                                          (Instr (ADDC (-128)) outHigh (outHigh, tmp2)
+                                                 (Instr (ADD 128) out (out, tmp)
+                                                        (Instr (ADDC (-128)) outHigh (outHigh, tmp) cont)))))))) cc ctx.
+  Proof.
+    intros; cbv [Prod.Mul256x256].
+    repeat (do_interp_step; cbn [spec MUL128LL MUL128UL MUL128LU MUL128UU ADD ADDC] in * ).
+
+    match goal with H : value_unused tmp _ |- _ => erewrite H end.
+    match goal with H : value_unused tmp2 _ |- _ => erewrite H end.
+    apply interp_state_equiv.
+    { rewrite !cc_overwrite_full.
+      f_equal.
+      subst. cbn - [Z.add Z.modulo Z.testbit Z.mul Z.shiftl Fancy.lower128 Fancy.upper128].
+      lia. }
+    { intros; cbv [reg_eqb].
+      repeat (break_match_step ltac:(fun _ => idtac); try congruence); try reflexivity; [ ].
+      subst. cbn - [Z.add Z.modulo Z.testbit Z.mul Z.shiftl Fancy.lower128 Fancy.upper128].
+      lia. }
+  Qed.
+End ProdEquiv.
+
+(* Lemmas to help prove that a fancy and prefancy expression have the
+same meaning -- should be replaced eventually with a proof of fancy
+passes in general. *)
+Module Fancy_PreFancy_Equiv.
+  Import Fancy.Registers.
+
+  Lemma interp_cast_mod_eq w u x: u = 2^w - 1 -> PreFancy.interp_cast_mod w r[0 ~> u] x = x mod 2^w.
+  Proof.
+    cbv [PreFancy.interp_cast_mod upper lower]; intros; subst.
+    rewrite !Z.eqb_refl.
+    reflexivity.
+  Qed.
+  Lemma interp_cast_mod_flag w x: PreFancy.interp_cast_mod w r[0 ~> 1] x = x mod 2.
+  Proof.
+    cbv [PreFancy.interp_cast_mod upper lower].
+    break_match; Z.ltb_to_lt; subst; try omega.
+    f_equal; lia.
+  Qed.
+
+  Lemma interp_equivZ {s} w u (Hu : u = 2^w-1) i rd regs e cc ctx idc args f :
+    (Fancy.spec i (Tuple.map ctx regs) cc
+     = PreFancy.interp_ident (d:=type.Z) w idc (Straightline.expr.interp_scalar (interp_cast:=PreFancy.interp_cast_mod w) args)) ->
+    ( let r := Fancy.spec i (Tuple.map ctx regs) cc in
+      Fancy.interp reg_eqb (2 ^ w) Fancy.cc_spec e
+                 (Fancy.CC.update (Fancy.writes_conditions i) r Fancy.cc_spec cc)
+                 (fun n : register => if reg_eqb n rd then r mod 2 ^ w else ctx n) =
+    PreFancy.interp (t:=type.Z) (interp_cast:=PreFancy.interp_cast_mod w) w (f (r mod 2 ^ w))) ->
+    Fancy.interp reg_eqb (2^w) Fancy.cc_spec (Fancy.Instr i rd regs e) cc ctx
+    = PreFancy.interp (t:=type.Z) (interp_cast:=PreFancy.interp_cast_mod w) w
+                      (@Straightline.expr.LetInAppIdentZ _ _ s _ (r[0~>2^w-1])%zrange idc args f).
+  Proof.
+    cbv zeta; intros spec_eq next_eq.
+    cbn [Fancy.interp PreFancy.interp].
+    rewrite next_eq.
+    rewrite <-spec_eq.
+    rewrite interp_cast_mod_eq by omega.
+    reflexivity.
+  Qed.
+
+  Lemma interp_equivZZ {s} w (Hw : 2 < 2 ^ w) u (Hu : u = 2^w - 1) i rd regs e cc ctx idc args f :
+    ((Fancy.spec i (Tuple.map ctx regs) cc) mod 2 ^ w
+     = fst (PreFancy.interp_ident (d:=type.Z*type.Z) w idc (Straightline.expr.interp_scalar (interp_cast:=PreFancy.interp_cast_mod w) args))) ->
+    ((if Fancy.cc_spec Fancy.CC.C(Fancy.spec i (Tuple.map ctx regs) cc) then 1 else 0)
+     = snd (PreFancy.interp_ident (d:=type.Z*type.Z) w idc (Straightline.expr.interp_scalar (interp_cast:=PreFancy.interp_cast_mod w) args)) mod 2) ->
+    ( let r := Fancy.spec i (Tuple.map ctx regs) cc in
+      Fancy.interp reg_eqb (2 ^ w) Fancy.cc_spec e
+                 (Fancy.CC.update (Fancy.writes_conditions i) r Fancy.cc_spec cc)
+                 (fun n : register => if reg_eqb n rd then r mod 2 ^ w else ctx n) =
+     PreFancy.interp (t:=type.Z) (interp_cast:=PreFancy.interp_cast_mod w) w
+                     (f (r mod 2 ^ w, if (Fancy.cc_spec Fancy.CC.C r) then 1 else 0))) ->
+    Fancy.interp reg_eqb (2^w) Fancy.cc_spec (Fancy.Instr i rd regs e) cc ctx
+    = PreFancy.interp (t:=type.Z) (interp_cast:=PreFancy.interp_cast_mod w) w
+                      (@Straightline.expr.LetInAppIdentZZ _ _ s _ (r[0~>u], r[0~>1])%zrange idc args f).
+  Proof.
+    cbv zeta; intros spec_eq1 spec_eq2 next_eq.
+    cbn [Fancy.interp PreFancy.interp].
+    cbv [Straightline.expr.interp_cast2]. cbn [fst snd].
+    rewrite next_eq.
+    rewrite interp_cast_mod_eq by omega.
+    rewrite interp_cast_mod_flag by omega.
+    rewrite <-spec_eq1, <-spec_eq2.
+    rewrite Z.mod_mod by omega.
+    reflexivity.
+  Qed.
+End Fancy_PreFancy_Equiv.
 
 Module BarrettReduction.
   (* TODO : generalize to multi-word and operate on (list Z) instead of T; maybe stop taking ops as context variables *)
@@ -10201,6 +11006,7 @@ Module Barrett256.
   Proof. Time solve_rbarrett_red machine_wordsize. Time Qed.
 
   Import PrintingNotations.
+  Set Printing Width 1000.
   Open Scope expr_scope.
 
   Print barrett_red256.
@@ -10209,21 +11015,16 @@ Module Barrett256.
      This is why their results are not cast (because the carry has range [-1~>0]). *)
   (*
 barrett_red256 =  fun var : type -> Type => λ x : var (type.type_primitive type.Z * type.type_primitive type.Z)%ctype,
-                expr_let x0 := SELM (x₂, 0,
-                               26959946667150639793205513449348445388433292963828203772348655992835) in
+                expr_let x0 := SELM (x₂, 0, 26959946667150639793205513449348445388433292963828203772348655992835) in
                 expr_let x1 := RSHI (0, x₂, 255) in
                 expr_let x2 := RSHI (x₂, x₁, 255) in
                 expr_let x3 := 79228162514264337589248983038 *₂₅₆ (uint128)(x2 >> 128) in
-                expr_let x4 := 79228162514264337589248983038 *₂₅₆
-                               ((uint128)(x2) & 340282366920938463463374607431768211455) in
+                expr_let x4 := 79228162514264337589248983038 *₂₅₆ ((uint128)(x2) & 340282366920938463463374607431768211455) in
                 expr_let x5 := 340282366841710300930663525764514709507 *₂₅₆ (uint128)(x2 >> 128) in
-                expr_let x6 := 340282366841710300930663525764514709507 *₂₅₆
-                               ((uint128)(x2) & 340282366920938463463374607431768211455) in
-                expr_let x7 := ADD_256 ((uint256)(((uint128)(x4) & 340282366920938463463374607431768211455) << 128),
-                               x6) in
-                expr_let x8 := ADDC_256 (x7₂, x3, (uint128)(x5 >> 128)) in
-                expr_let x9 := ADD_256 ((uint256)(((uint128)(x5) & 340282366920938463463374607431768211455) << 128),
-                               x7₁) in
+                expr_let x6 := 340282366841710300930663525764514709507 *₂₅₆ ((uint128)(x2) & 340282366920938463463374607431768211455) in
+                expr_let x7 := ADD_256 ((uint256)(((uint128)(x5) & 340282366920938463463374607431768211455) << 128), x6) in
+                expr_let x8 := ADDC_256 (x7₂, (uint128)(x5 >> 128), x3) in
+                expr_let x9 := ADD_256 ((uint256)(((uint128)(x4) & 340282366920938463463374607431768211455) << 128), x7₁) in
                 expr_let x10 := ADDC_256 (x9₂, (uint128)(x4 >> 128), x8₁) in
                 expr_let x11 := ADD_256 (x2, x10₁) in
                 expr_let x12 := ADDC_128 (x11₂, 0, x1) in
@@ -10232,27 +11033,17 @@ barrett_red256 =  fun var : type -> Type => λ x : var (type.type_primitive type
                 expr_let x15 := RSHI (x14₁, x13₁, 1) in
                 expr_let x16 := 340282366841710300967557013911933812736 *₂₅₆ (uint128)(x15 >> 128) in
                 expr_let x17 := 79228162514264337593543950335 *₂₅₆ (uint128)(x15 >> 128) in
-                expr_let x18 := 340282366841710300967557013911933812736 *₂₅₆
-                                ((uint128)(x15) & 340282366920938463463374607431768211455) in
-                expr_let x19 := 79228162514264337593543950335 *₂₅₆
-                                ((uint128)(x15) & 340282366920938463463374607431768211455) in
-                expr_let x20 := ADD_256 ((uint256)(((uint128)(x17) & 340282366920938463463374607431768211455) << 128),
-                                x19) in
-                expr_let x21 := ADDC_256 (x20₂, x16, (uint128)(x18 >> 128)) in
-                expr_let x22 := ADD_256 ((uint256)(((uint128)(x18) & 340282366920938463463374607431768211455) << 128),
-                                x20₁) in
+                expr_let x18 := 340282366841710300967557013911933812736 *₂₅₆ ((uint128)(x15) & 340282366920938463463374607431768211455) in
+                expr_let x19 := 79228162514264337593543950335 *₂₅₆ ((uint128)(x15) & 340282366920938463463374607431768211455) in
+                expr_let x20 := ADD_256 ((uint256)(((uint128)(x18) & 340282366920938463463374607431768211455) << 128), x19) in
+                expr_let x21 := ADDC_256 (x20₂, (uint128)(x18 >> 128), x16) in
+                expr_let x22 := ADD_256 ((uint256)(((uint128)(x17) & 340282366920938463463374607431768211455) << 128), x20₁) in
                 expr_let x23 := ADDC_256 (x22₂, (uint128)(x17 >> 128), x21₁) in
-                expr_let x24 := Z.add_get_carry_concrete
-                                  115792089237316195423570985008687907853269984665640564039457584007913129639936 @@
-                                (Z.opp @@ (fst @@ x22), x₁) in
-                expr_let x25 := Z.add_with_get_carry_concrete
-                                  115792089237316195423570985008687907853269984665640564039457584007913129639936 @@
-                                (x24₂, Z.opp @@ (fst @@ x23), x₂) in
-                expr_let x26 := SELL (x25₁, 0,
-                                115792089210356248762697446949407573530086143415290314195533631308867097853951) in
+                expr_let x24 := Z.add_get_carry_concrete 115792089237316195423570985008687907853269984665640564039457584007913129639936 @@ (Z.opp @@ (fst @@ x22), x₁) in
+                expr_let x25 := Z.add_with_get_carry_concrete 115792089237316195423570985008687907853269984665640564039457584007913129639936 @@ (x24₂, Z.opp @@ (fst @@ x23), x₂) in
+                expr_let x26 := SELL (x25₁, 0, 115792089210356248762697446949407573530086143415290314195533631308867097853951) in
                 expr_let x27 := Z.cast uint256 @@ (fst @@ SUB_256 (x24₁, x26)) in
-                ADDM (x27, 0,
-                115792089210356248762697446949407573530086143415290314195533631308867097853951)
+                ADDM (x27, 0, 115792089210356248762697446949407573530086143415290314195533631308867097853951)
      : Expr (type.uncurry (type.type_primitive type.Z -> type.type_primitive type.Z -> type.type_primitive type.Z))
   *)
 
@@ -10274,9 +11065,9 @@ barrett_red256 =  fun var : type -> Type => λ x : var (type.type_primitive type
     mulhl@(y3, RegMuLow, $y1);
     mullh@(y4, RegMuLow, $y1);
     mulll@(y5, RegMuLow, $y1);
-    add@(y6, $y5, $y3, 128);
+    add@(y6, $y5, $y4, 128);
     addc@(y7, carry{$y6}, $y2, $y4, -128);
-    add@(y8, $y6, $y4, 128);
+    add@(y8, $y6, $y3, 128);
     addc@(y9, carry{$y8}, $y7, $y3, -128);
     add@(y10, $y1, $y9, 0);
     addc@(y11, carry{$y10}, RegZero, $y0, 0); #128
@@ -10287,9 +11078,9 @@ barrett_red256 =  fun var : type -> Type => λ x : var (type.type_primitive type
     mullh@(y16, RegMod, $y14);
     mulhl@(y17, RegMod, $y14);
     mulll@(y18, RegMod, $y14);
-    add@(y19, $y18, $y16, 128);
+    add@(y19, $y18, $y17, 128);
     addc@(y20, carry{$y19}, $y15, $y17, -128);
-    add@(y21, $y19, $y17, 128);
+    add@(y21, $y19, $y16, 128);
     addc@(_, carry{$y21}, $y20, $y16, -128);
     Straightline.expr.Scalar (Straightline.expr.Primitive (-1))            
   *)
@@ -10706,7 +11497,7 @@ Module MontgomeryReduction.
 
     Definition montred' (lo_hi : (Z * Z)) :=
       dlet_nd y := nth_default 0 (BaseConversion.widemul_inlined Zlog2R n nout (fst lo_hi) N') 0  in
-      dlet_nd t1_t2 := (BaseConversion.widemul_inlined Zlog2R n nout y N) in
+      dlet_nd t1_t2 := (BaseConversion.widemul_inlined_reverse Zlog2R n nout N y) in
       dlet_nd sum_carry := Rows.add (weight Zlog2R 1) 2 [fst lo_hi; snd lo_hi] t1_t2 in
       dlet_nd y' := Z.zselect (snd sum_carry) 0 N in
       dlet_nd lo''_carry := Z.sub_get_borrow_full R (nth_default 0 (fst sum_carry) 1) y' in
@@ -10734,6 +11525,9 @@ Module MontgomeryReduction.
     Local Lemma eval2 x y : eval w 2 [x;y] = x + R * y.
     Proof. cbn. change_weight. ring. Qed.
 
+    Hint Rewrite BaseConversion.widemul_inlined_reverse_correct BaseConversion.widemul_inlined_correct
+         using (autorewrite with widemul push_nth_default; solve [solve_range]) : widemul.
+
     Lemma montred'_eq lo_hi T (HT_range: 0 <= T < R * N)
           (Hlo: fst lo_hi = T mod R) (Hhi: snd lo_hi = T / R):
       montred' lo_hi = reduce_via_partial N R N' T.
@@ -10741,10 +11535,9 @@ Module MontgomeryReduction.
       rewrite <-reduce_via_partial_alt_eq by nia.
       cbv [montred' partial_reduce_alt reduce_via_partial_alt prereduce Let_In].
       rewrite Hlo, Hhi.
-      assert (0 <= T mod R * N' < w 2) by (solve_range).
+      assert (0 <= (T mod R) * N' < w 2) by  (solve_range).
 
-      rewrite !BaseConversion.widemul_inlined_correct
-        by (rewrite ?BaseConversion.widemul_inlined_correct; autorewrite with push_nth_default; solve_range).
+      autorewrite with widemul.
       rewrite Rows.add_partitions, Rows.add_div by (distr_length; apply wprops; omega).
       rewrite R_two_pow.
       cbv [Rows.partition seq]. rewrite !eval2.
@@ -10757,7 +11550,8 @@ Module MontgomeryReduction.
                       let P := fresh "H" in assert (x = y) as P; [|rewrite P; reflexivity] end.
 
       autorewrite with zsimplify.
-      break_match; try reflexivity; autorewrite with ltb_to_lt in *; rewrite Z.div_small_iff in * by omega;
+      rewrite (Z.mul_comm (((T mod R) * N') mod R) N) in *.
+      break_match; try reflexivity; Z.ltb_to_lt; rewrite Z.div_small_iff in * by omega;
         repeat match goal with
                | _ => progress autorewrite with zsimplify_fast
                | |- context [?x mod (R * R)] =>
@@ -10842,6 +11636,7 @@ Module Montgomery256.
   Definition N := Eval lazy in (2^256-2^224+2^192+2^96-1).
   Definition N':= (115792089210356248768974548684794254293921932838497980611635986753331132366849).
   Definition R := Eval lazy in (2^256).
+  Definition R' := 115792089183396302114378112356516095823261736990586219612555396166510339686400.
   Definition machine_wordsize := 256.
 
   Derive montred256
@@ -10855,6 +11650,7 @@ Module Montgomery256.
          SuchThat (montred256_prefancy = montred256_prefancy' type.interp)
          As montred256_prefancy_eq.
   Proof. lazy - [type.interp]; reflexivity. Qed.
+
 
   Lemma montred'_correct_specialized R' (R'_correct : Z.equiv_modulo N (R * R') 1) :
     forall (lo hi : Z),
@@ -10933,14 +11729,14 @@ Module Montgomery256.
     | |- context [PreFancy.ok_expr] => constructor; cbn [fst snd]; repeat ok_expr_step'
     end; intros; cbn [Nat.max].
 
-  Lemma montred256_prefancy_correct R' (R'_correct : Z.equiv_modulo N (R * R') 1) :
+  Lemma montred256_prefancy_correct :
     forall (lo hi : Z) dummy_arrow,
       0 <= lo < R -> 0 <= hi < R -> 0 <= lo + R * hi < R * N ->
-      @PreFancy.interp machine_wordsize type.Z (montred256_prefancy (lo,hi) dummy_arrow) = ((lo + R * hi) * R') mod N.
+      @PreFancy.interp machine_wordsize (PreFancy.interp_cast_mod machine_wordsize) type.Z (montred256_prefancy (lo,hi) dummy_arrow) = ((lo + R * hi) * R') mod N.
   Proof.
     intros. rewrite montred256_prefancy_eq; cbv [montred256_prefancy'].
     erewrite PreFancy.of_Expr_correct.
-    { apply montred256_correct_full; assumption. }
+    { apply montred256_correct_full; try assumption; reflexivity. }
     { reflexivity. }
     { lazy; reflexivity. }
     { lazy; reflexivity. }
@@ -10950,9 +11746,297 @@ Module Montgomery256.
       repeat (ok_expr_step; [ ]).
       ok_expr_step.
       lazy; congruence.
+      constructor.
       constructor. }
     { lazy. omega. }
    Qed.
+
+  Definition montred256_fancy' (lo hi RegMod RegPInv RegZero error : positive) :=
+    Fancy.of_Expr 3%positive
+                  (fun z => if z =? N then Some RegMod else if z =? N' then Some RegPInv else if z =? 0 then Some RegZero else None)
+                  [N;N']
+                  montred256
+                  (lo, hi)%positive
+                  (fun _ _ => tt)
+                  error.
+  Derive montred256_fancy
+         SuchThat (forall RegMod RegPInv RegZero,
+                      montred256_fancy RegMod RegPInv RegZero = montred256_fancy' RegMod RegPInv RegZero)
+         As montred256_fancy_eq.
+  Proof.
+    intros.
+    lazy - [Fancy.ADD Fancy.ADDC Fancy.SUB
+                      Fancy.MUL128LL Fancy.MUL128LU Fancy.MUL128UL Fancy.MUL128UU
+                      Fancy.RSHI Fancy.SELC Fancy.SELM Fancy.SELL Fancy.ADDM].
+    reflexivity.
+  Qed.
+
+  Import Fancy.Registers.
+
+  Definition montred256_alloc' lo hi RegPInv :=
+    fun errorP errorR =>
+    Fancy.allocate register
+                   positive Pos.eqb
+                   errorR
+                   (montred256_fancy 1000%positive 1001%positive 1002%positive 1003%positive 1004%positive errorP)
+                   [r2;r3;r4;r5;r6;r7;r8;r9;r10;r11;r12;r13;r14;r15;r16;r17;r18;r19;r20]
+                   (fun n => if n =? 1000 then lo
+                             else if n =? 1001 then hi
+                                  else if n =? 1002 then RegMod
+                                       else if n =? 1003 then RegPInv
+                                            else if n =? 1004 then RegZero
+                                                 else errorR).
+  Derive montred256_alloc
+         SuchThat (montred256_alloc = montred256_alloc')
+         As montred256_alloc_eq.
+  Proof.
+    intros.
+    cbv [montred256_alloc' montred256_fancy].
+    cbn. subst montred256_alloc.
+    reflexivity.
+  Qed.
+
+  (* TODO : move *)
+  Lemma mulll_comm rd x y cont cc ctx :
+    ProdEquiv.interp256 (Fancy.Instr Fancy.MUL128LL rd (x, y) cont) cc ctx = ProdEquiv.interp256 (Fancy.Instr Fancy.MUL128LL rd (y, x) cont) cc ctx.
+  Proof. rewrite !ProdEquiv.interp_step. cbn - [Fancy.interp]. rewrite Z.mul_comm. reflexivity. Qed.
+
+  Lemma mulhh_comm rd x y cont cc ctx :
+    ProdEquiv.interp256 (Fancy.Instr Fancy.MUL128UU rd (x, y) cont) cc ctx = ProdEquiv.interp256 (Fancy.Instr Fancy.MUL128UU rd (y, x) cont) cc ctx.
+  Proof. rewrite !ProdEquiv.interp_step. cbn - [Fancy.interp]. rewrite Z.mul_comm. reflexivity. Qed.
+
+  Lemma mullh_mulhl rd x y cont cc ctx :
+    ProdEquiv.interp256 (Fancy.Instr Fancy.MUL128LU rd (x, y) cont) cc ctx = ProdEquiv.interp256 (Fancy.Instr Fancy.MUL128UL rd (y, x) cont) cc ctx.
+  Proof. rewrite !ProdEquiv.interp_step. cbn - [Fancy.interp]. rewrite Z.mul_comm. reflexivity. Qed.
+
+  Lemma add_comm rd x y cont cc ctx :
+    0 <= ctx x < 2^256 ->
+    0 <= ctx y < 2^256 ->
+    ProdEquiv.interp256 (Fancy.Instr (Fancy.ADD 0) rd (x, y) cont) cc ctx = ProdEquiv.interp256 (Fancy.Instr (Fancy.ADD 0) rd (y, x) cont) cc ctx.
+  Proof.
+    intros; rewrite !ProdEquiv.interp_step. cbn - [Fancy.interp]. rewrite Z.add_comm.
+    rewrite !(Z.mod_small (ctx _)) by (cbn in *; omega). reflexivity.
+  Qed.
+
+  Lemma addc_comm rd x y cont cc ctx :
+    0 <= ctx x < 2^256 ->
+    0 <= ctx y < 2^256 ->
+    ProdEquiv.interp256 (Fancy.Instr (Fancy.ADDC 0) rd (x, y) cont) cc ctx = ProdEquiv.interp256 (Fancy.Instr (Fancy.ADDC 0) rd (y, x) cont) cc ctx.
+  Proof.
+    intros; rewrite !ProdEquiv.interp_step. cbn - [Fancy.interp]. rewrite (Z.add_comm (ctx x)).
+    rewrite !(Z.mod_small (ctx _)) by (cbn in *; omega). reflexivity.
+  Qed.
+
+  SearchAbout reg_eqb.
+
+  Local Ltac push_value_unused :=
+    repeat match goal with
+           | |- ~ In _ _ => cbn; intuition; congruence
+           | _ => apply ProdEquiv.value_unused_overwrite
+           | _ => apply ProdEquiv.value_unused_skip; [ | congruence | ]
+           | _ => apply ProdEquiv.value_unused_ret; congruence
+           end.
+
+  Local Ltac remember_single_result :=
+    match goal with |- context [(Fancy.spec ?i ?args ?cc) mod ?w] =>
+                    let x := fresh "x" in
+                    let y := fresh "y" in
+                    let Heqx := fresh "Heqx" in
+                    remember (Fancy.spec i args cc) as x eqn:Heqx;
+                    remember (x mod w) as y
+    end.
+  Local Ltac step_both_sides :=
+    match goal with |- ProdEquiv.interp256 (Fancy.Instr ?i ?rd1 ?args1 _) _ ?ctx1 = ProdEquiv.interp256 (Fancy.Instr ?i ?rd2 ?args2 _) _ ?ctx2 =>
+                    rewrite (ProdEquiv.interp_step i rd1 args1); rewrite (ProdEquiv.interp_step i rd2 args2);
+                    cbn - [Fancy.interp Fancy.spec];
+                    repeat progress rewrite ?reg_eqb_neq, ?reg_eqb_refl by congruence;
+                    remember_single_result;
+                    lazymatch goal with
+                    | |- context [Fancy.spec i _ _] =>
+                      let Heqa1 := fresh in
+                      let Heqa2 := fresh in
+                      remember (Tuple.map (n:=i.(Fancy.num_source_regs)) ctx1 args1) eqn:Heqa1;
+                      remember (Tuple.map (n:=i.(Fancy.num_source_regs)) ctx2 args2) eqn:Heqa2;
+                      cbn in Heqa1; cbn in Heqa2;
+                      repeat progress rewrite ?reg_eqb_neq, ?reg_eqb_refl in Heqa1 by congruence;
+                      repeat progress rewrite ?reg_eqb_neq, ?reg_eqb_refl in Heqa2 by congruence;
+                      let a1 := match type of Heqa1 with _ = ?a1 => a1 end in
+                      let a2 := match type of Heqa2 with _ = ?a2 => a2 end in
+                      (fail 1 "arguments to " i " do not match; LHS has " a1 " and RHS has " a2)
+                    | _ => idtac
+                    end
+    end.
+
+  Local Ltac solve_bounds :=
+    match goal with
+    | H : ?a = ?b mod ?c |- 0 <= ?a < ?c => rewrite H; apply Z.mod_pos_bound; omega
+    | _ => assumption
+    end.
+
+  Lemma montred256_alloc_equivalent errorP errorR cc_start_state start_context :
+    forall lo hi y t1 t2 scratch RegPInv extra_reg,
+      NoDup [lo; hi; y; t1; t2; scratch; RegPInv; extra_reg; RegMod; RegZero] ->
+      0 <= start_context lo < R ->
+      0 <= start_context hi < R ->
+      0 <= start_context RegPInv < R ->
+      ProdEquiv.interp256 (montred256_alloc r0 r1 r30 errorP errorR) cc_start_state
+                          (fun r => if reg_eqb r r0
+                                    then start_context lo
+                                    else if reg_eqb r r1
+                                         then start_context hi
+                                         else if reg_eqb r r30
+                                              then start_context RegPInv
+                                              else start_context r)
+    = ProdEquiv.interp256 (Prod.MontRed256 lo hi y t1 t2 scratch RegPInv) cc_start_state start_context.
+  Proof.
+    intros. cbv [R] in *.
+    cbv [Prod.MontRed256 montred256_alloc].
+
+    (* Extract proofs that no registers are equal to each other *)
+    repeat match goal with
+           | H : NoDup _ |- _ => inversion H; subst; clear H
+           | H : ~ In _ _ |- _ => cbv [In] in H
+           | H : ~ (_ \/ _) |- _ => apply Decidable.not_or in H; destruct H
+           | H : ~ False |- _ => clear H
+           end.
+
+    rewrite ProdEquiv.interp_Mul256 with (tmp2:=extra_reg) by (congruence || push_value_unused).
+
+    step_both_sides.
+    step_both_sides.
+    rewrite mulll_comm. step_both_sides.
+    step_both_sides.
+    step_both_sides.
+
+    rewrite ProdEquiv.interp_Mul256x256 with (tmp2:=extra_reg) by (congruence || push_value_unused).
+
+    rewrite mulll_comm. step_both_sides.
+    step_both_sides.
+    step_both_sides.
+    rewrite mulhh_comm. step_both_sides.
+    step_both_sides.
+    step_both_sides.
+    step_both_sides.
+    step_both_sides.
+
+
+    rewrite add_comm by (cbn; solve_bounds). step_both_sides.
+    rewrite addc_comm by (cbn; solve_bounds). step_both_sides.
+    step_both_sides.
+    step_both_sides.
+    step_both_sides.
+
+    cbn; repeat progress rewrite ?reg_eqb_neq, ?reg_eqb_refl by congruence.
+    reflexivity.
+  Qed.
+
+  Import Fancy_PreFancy_Equiv.
+
+  Definition interp_equivZZ_256 {s} :=
+    @interp_equivZZ s 256 ltac:(cbv; congruence) 115792089237316195423570985008687907853269984665640564039457584007913129639935 ltac:(reflexivity).
+  Definition interp_equivZ_256 {s} :=
+    @interp_equivZ s 256 115792089237316195423570985008687907853269984665640564039457584007913129639935 ltac:(reflexivity).
+
+  Local Ltac simplify_op_equiv start_ctx :=
+    cbn - [Fancy.spec PreFancy.interp_ident Fancy.cc_spec];
+    repeat match goal with H : start_ctx _ = _ |- _ => rewrite H end;
+    cbv - [
+      Z.add_with_get_carry_full
+        Z.add_get_carry_full Z.sub_get_borrow_full
+        Z.le Z.ltb Z.leb Z.geb Z.eqb Z.land Z.shiftr Z.shiftl
+        Z.add Z.mul Z.div Z.sub Z.modulo Z.testbit Z.pow Z.ones
+        fst snd]; cbn [fst snd];
+    try (replace (2 ^ (256 / 2) - 1) with (Z.ones 128) by reflexivity; rewrite !Z.land_ones by omega);
+    autorewrite with to_div_mod; rewrite ?Z.mod_mod, <-?Z.testbit_spec' by omega;
+    repeat match goal with
+           | H : 0 <= ?x < ?m |- context [?x mod ?m] => rewrite (Z.mod_small x m) by apply H
+           | |- context [?x <? 0] => rewrite (proj2 (Z.ltb_ge x 0)) by (break_match; Z.zero_bounds)
+           | _ => rewrite Z.mod_small with (b:=2) by (break_match; omega)
+           | |- context [ (if Z.testbit ?a ?n then 1 else 0) + ?b + ?c] =>
+             replace ((if Z.testbit a n then 1 else 0) + b + c) with (b + c + (if Z.testbit a n then 1 else 0)) by ring
+           end.
+
+  Local Ltac solve_nonneg ctx :=
+    match goal with x := (Fancy.spec _ _ _) |- _ => subst x end;
+    simplify_op_equiv ctx; Z.zero_bounds.
+
+  Local Ltac generalize_result :=
+    let v := fresh "v" in intro v; generalize v; clear v; intro v.
+
+  Local Ltac generalize_result_nonneg ctx :=
+    let v := fresh "v" in
+    let v_nonneg := fresh "v_nonneg" in
+    intro v; assert (0 <= v) as v_nonneg; [solve_nonneg ctx |generalize v v_nonneg; clear v v_nonneg; intros v v_nonneg].
+
+  Local Ltac step ctx :=
+    match goal with
+    | |- Fancy.interp _ _ _ (Fancy.Instr (Fancy.ADD _) _ _ (Fancy.Instr (Fancy.ADDC _) _ _ _)) _ _ = _ =>
+      apply interp_equivZZ_256; [ simplify_op_equiv ctx | simplify_op_equiv ctx | generalize_result_nonneg ctx]
+    | _ => apply interp_equivZ_256; [simplify_op_equiv ctx | generalize_result]
+    | _ => apply interp_equivZZ_256; [ simplify_op_equiv ctx | simplify_op_equiv ctx | generalize_result]
+    end.
+
+  (* TODO: move this lemma to ZUtil *)
+  Lemma testbit_neg_eq_if x y n :
+    0 <= n ->
+    0 <= x < 2 ^ n ->
+    0 <= y < 2 ^ n ->
+    Z.b2z (if (x - y) <? 0 then true else Z.testbit (x - y) n) = - ((x - y) / 2 ^ n) mod 2.
+  Proof.
+    intros. rewrite Z.sub_pos_bound_div_eq by omega.
+    break_innermost_match; Z.ltb_to_lt; try lia; try reflexivity; [ ].
+    rewrite Z.testbit_eqb, Z.div_between_0_if by omega.
+    break_innermost_match; Z.ltb_to_lt; try lia; reflexivity.
+  Qed.
+
+  Lemma prod_montred256_correct :
+    forall (cc_start_state : Fancy.CC.state) (* starting carry flags can be anything *)
+           (start_context : register -> Z)   (* starting register values *)
+           (lo hi y t1 t2 scratch RegPInv extra_reg : register), (* registers to use in computation *)
+      NoDup [lo; hi; y; t1; t2; scratch; RegPInv; extra_reg; RegMod; RegZero] -> (* registers must be distinct *)
+      start_context RegPInv = N' ->  (* RegPInv needs to hold the inverse of the modulus *)
+      start_context RegMod = N ->    (* RegMod needs to hold the modulus *)
+      start_context RegZero = 0 ->   (* RegZero needs to hold zero *)
+      (0 <= start_context lo < R) -> (* value in lo is in bounds (R=2^256) *)
+      (0 <= start_context hi < R) -> (* value in hi is in bounds (R=2^256) *)
+      let x := (start_context lo) + R * (start_context hi) in (* x is the input (split into two registers) *)
+      (0 <= x < R * N) -> (* input precondition *)
+      (ProdEquiv.interp256 (Prod.MontRed256 lo hi y t1 t2 scratch RegPInv) cc_start_state start_context = (x * R') mod N).
+  Proof.
+    intros. subst x. cbv [N R N'] in *.
+    rewrite <-montred256_prefancy_correct with (dummy_arrow := fun s d _ => DefaultValue.type.default) by auto.
+    rewrite <-montred256_alloc_equivalent with (errorR := RegZero) (errorP := 1%positive) (extra_reg:=extra_reg)
+      by (cbv [R]; auto with omega).
+    cbv [ProdEquiv.interp256].
+    cbv [montred256_alloc montred256_prefancy].
+
+    step start_context; [ reflexivity | ].
+    step start_context; [ reflexivity | ].
+    step start_context; [ reflexivity | ].
+    step start_context; [ reflexivity | reflexivity | ].
+    step start_context; [ reflexivity | reflexivity | ].
+    step start_context; [ reflexivity | ].
+    step start_context; [ reflexivity | ].
+    step start_context; [ reflexivity | ].
+    step start_context; [ reflexivity | ].
+    step start_context; [ reflexivity | reflexivity | ].
+    step start_context; [ reflexivity | reflexivity | ].
+    step start_context; [ reflexivity | reflexivity | ].
+    step start_context; [ reflexivity | reflexivity | ].
+
+    step start_context; [ reflexivity | reflexivity | ].
+    step start_context; [ reflexivity | reflexivity | ].
+    step start_context; [ break_innermost_match; Z.ltb_to_lt; omega | ].
+    step start_context; [ reflexivity | | ].
+    {
+      let r := eval cbv in (2^256) in replace (2^256) with r by reflexivity.
+      rewrite !Z.shiftl_0_r, !Z.mod_mod by omega.
+      apply testbit_neg_eq_if;
+        let r := eval cbv in (2^256) in replace (2^256) with r by reflexivity;
+        auto using Z.mod_pos_bound with omega. }
+    step start_context; [ break_innermost_match; Z.ltb_to_lt; omega | ].
+    reflexivity.
+  Qed.
 
   Import PrintingNotations.
   Set Printing Width 10000.
@@ -10963,15 +12047,15 @@ montred256 = fun var : type -> Type => (λ x : var (type.type_primitive type.Z *
     expr_let x0 := 79228162514264337593543950337 *₂₅₆ (uint128)(x₁ >> 128) in
     expr_let x1 := 340282366841710300986003757985643364352 *₂₅₆ ((uint128)(x₁) & 340282366920938463463374607431768211455) in
     expr_let x2 := 79228162514264337593543950337 *₂₅₆ ((uint128)(x₁) & 340282366920938463463374607431768211455) in
-    expr_let x3 := ADD_256 ((uint256)(((uint128)(x0) & 340282366920938463463374607431768211455) << 128), x2) in
-    expr_let x4 := ADD_256 ((uint256)(((uint128)(x1) & 340282366920938463463374607431768211455) << 128), x3₁) in
-    expr_let x5 := 340282366841710300967557013911933812736 *₂₅₆ (uint128)(x4₁ >> 128) in
+    expr_let x3 := ADD_256 ((uint256)(((uint128)(x1) & 340282366920938463463374607431768211455) << 128), x2) in
+    expr_let x4 := ADD_256 ((uint256)(((uint128)(x0) & 340282366920938463463374607431768211455) << 128), x3₁) in
+    expr_let x5 := 79228162514264337593543950335 *₂₅₆ ((uint128)(x4₁) & 340282366920938463463374607431768211455) in
     expr_let x6 := 79228162514264337593543950335 *₂₅₆ (uint128)(x4₁ >> 128) in
     expr_let x7 := 340282366841710300967557013911933812736 *₂₅₆ ((uint128)(x4₁) & 340282366920938463463374607431768211455) in
-    expr_let x8 := 79228162514264337593543950335 *₂₅₆ ((uint128)(x4₁) & 340282366920938463463374607431768211455) in
-    expr_let x9 := ADD_256 ((uint256)(((uint128)(x6) & 340282366920938463463374607431768211455) << 128), x8) in
-    expr_let x10 := ADDC_256 (x9₂, x5, (uint128)(x7 >> 128)) in
-    expr_let x11 := ADD_256 ((uint256)(((uint128)(x7) & 340282366920938463463374607431768211455) << 128), x9₁) in
+    expr_let x8 := 340282366841710300967557013911933812736 *₂₅₆ (uint128)(x4₁ >> 128) in
+    expr_let x9 := ADD_256 ((uint256)(((uint128)(x7) & 340282366920938463463374607431768211455) << 128), x5) in
+    expr_let x10 := ADDC_256 (x9₂, (uint128)(x7 >> 128), x8) in
+    expr_let x11 := ADD_256 ((uint256)(((uint128)(x6) & 340282366920938463463374607431768211455) << 128), x9₁) in
     expr_let x12 := ADDC_256 (x11₂, (uint128)(x6 >> 128), x10₁) in
     expr_let x13 := ADD_256 (x11₁, x₁) in
     expr_let x14 := ADDC_256 (x13₂, x12₁, x₂) in
@@ -10989,23 +12073,24 @@ montred256 = fun var : type -> Type => (λ x : var (type.type_primitive type.Z *
   (*
    mulhl@(y0, RegPInv, $x₁);
    mulll@(y1, RegPInv, $x₁);
-   add@(y2, $y1, $y, 128);
-   add@(y3, $y2, $y0, 128);
-   mulhh@(y4, RegMod, $y3);
+   add@(y2, $y1, $y0, 128);
+   add@(y3, $y2, $y, 128);
+   mulll@(y4, RegMod, $y3);
    mullh@(y5, RegMod, $y3);
    mulhl@(y6, RegMod, $y3);
-   mulll@(y7, RegMod, $y3);
-   add@(y8, $y7, $y5, 128);
-   addc@(y9, carry{$y8}, $y4, $y6, -128);
-   add@(y10, $y8, $y6, 128);
+   mulhh@(y7, RegMod, $y3);
+   add@(y8, $y4, $y6, 128);
+   addc@(y9, carry{$y8}, $y7, $y6, -128);
+   add@(y10, $y8, $y5, 128);
    addc@(y11, carry{$y10}, $y9, $y5, -128);
    add@(y12, $y10, $x₁, 0);
    addc@(y13, carry{$y12}, $y11, $x₂, 0);
    selc@(y14, carry{$y13}, RegZero, RegMod);
    sub@(y15, $y13, $y14, 0);
    addm@(y16, $y15, RegZero, RegMod);
-   ret $y16         
+   ret $y16
   *)
+
 End Montgomery256.
 
 (* Extra-specialized ad-hoc pretty-printing *)
@@ -11139,6 +12224,39 @@ Module FancyPrintingNotations.
   *)
 End FancyPrintingNotations.
 
+
+Local Notation "i rd x y ; cont" := (Fancy.Instr i rd (x, y) cont) (at level 40, cont at level 200, format "i  rd  x  y ; '//' cont").
+Local Notation "i rd x y z ; cont" := (Fancy.Instr i rd (x, y, z) cont) (at level 40, cont at level 200, format "i  rd  x  y  z ; '//' cont").
+
+Import Fancy.Registers.
+Import Fancy.
+Eval cbv beta iota delta [Prod.MontRed256 Prod.Mul256 Prod.Mul256x256] in Prod.MontRed256.
+(*
+     = fun lo hi y t1 t2 scratch RegPInv : register =>
+       MUL128LL y lo RegPInv;
+       MUL128UL t1 lo RegPInv;
+       ADD 128 y y t1;
+       MUL128LU t1 lo RegPInv;
+       ADD 128 y y t1;
+       MUL128LL t1 y RegMod;
+       MUL128UU t2 y RegMod;
+       MUL128UL scratch y RegMod;
+       ADD 128 t1 t1 scratch;
+       ADDC (-128) t2 t2 scratch;
+       MUL128LU scratch y RegMod;
+       ADD 128 t1 t1 scratch;
+       ADDC (-128) t2 t2 scratch;
+       ADD 0 lo lo t1;
+       ADDC 0 hi hi t2;
+       SELC y RegMod RegZero;
+       SUB 0 lo hi y;
+       ADDM lo lo RegZero RegMod;
+       Ret lo
+ *)
+Import Montgomery256.
+Check Montgomery256.prod_montred256_correct.
+(* Print Assumptions Montgomery256.prod_montred256_correct. *)
+
 Import FancyPrintingNotations.
 Local Open Scope expr_scope.
 
@@ -11177,26 +12295,4 @@ expr_let x25 := Z.add_with_get_carry_concrete
 c.Sell($x26, $x25_lo, RegZero, RegMod);
 c.Sub($x27, $x24_lo, $x26);
 c.AddM($ret, $x27, RegZero, RegMod);
-*)
-
-Print Montgomery256.montred256.
-(*
-c.Mul128x128($x0, c.Lower(RegPinv), c.Upper($x_lo));
-c.Mul128x128($x1, c.Upper(RegPinv), c.Lower($x_lo));
-c.Mul128x128($x2, c.Lower(RegPinv), c.Lower($x_lo));
-c.Add256($x3, (c.Lower($x0) << 128), $x2);
-c.Add256($x4, (c.Lower($x1) << 128), $x3_lo);
-c.Mul128x128($x5, c.Upper(RegMod), c.Upper($x4_lo));
-c.Mul128x128($x6, c.Lower(RegMod), c.Upper($x4_lo));
-c.Mul128x128($x7, c.Upper(RegMod), c.Lower($x4_lo));
-c.Mul128x128($x8, c.Lower(RegMod), c.Lower($x4_lo));
-c.Add256($x9, (c.Lower($x6) << 128), $x8);
-c.Addc256($x10, $x9_hi, $x5, c.Upper($x7));
-c.Add256($x11, (c.Lower($x7) << 128), $x9_lo);
-c.Addc256($x12, $x11_hi, c.Upper($x6), $x10_lo);
-c.Add256($x13, $x11_lo, $x_lo);
-c.Addc256($x14, $x13_hi, $x12_lo, $x_hi);
-c.Selc($x15, $x14_hi, RegZero, RegMod);
-c.Sub($x16, $x14_lo, $x15);
-c.AddM($ret, $x16_lo, RegZero, RegMod);
  *)
